# Solving Quadratic Equations using Quadratic Formula

The equation of a quadratic formula is in the form

```
ax^2 + bx + c = 0
```

The equation has to be equal to zero.


a is always the coefficient of the highest term, b is the coefficient of the next highest term, and c is represented by the constant.


```
2x^2 + 2x - 5 = 0
Where a = 2, b = 2, c = -5
```

The **Quadratic Equation** is represented by:

```
x = (-b +- sqrt(b^2 - 4ac)) / 2a
```


```
Solution:
x = (-2 +- sqrt(2^2 - 4(2)(-5))) / 2(2)
x = (-2 +- sqrt(4 + 40)) / 4
x = (-2 +- sqrt(44)) / 4
x = (-2 +- 2*sqrt(11))/ 4
x = (-1 +- sqrt(11)) / 2
```
